

Ramp-up Mathematics — Analysis

Extra Homework Sheet

Here are some more exercises you can do to prepare for the exam.

- Recall that for a square matrix $M \in \mathbb{R}^{n \times n}$ it holds that $\text{Tr}(M) := \sum_{k=1}^n M_{kk}$ and that the inner product for matrices $A, B \in \mathbb{R}^{m \times n}$ is defined by $\langle A, B \rangle := \text{Tr}(AB^T)$.
Prove or disprove that for this inner product it holds that $\langle A, B \rangle = \langle A^T, B^T \rangle$

- Define $F : \mathbb{R}^{m \times n} \rightarrow \mathbb{R}$ by $F(R) = \text{Tr}(RR^T)$.

(a) Calculate the derivative $DF(R)[H]$! (You can equip $\mathbb{R}^{m \times n}$ with any of your favorite norms. Recall that all norms on finite-dimensional vector spaces are equivalent to each other.)

(b) What is the gradient $\nabla F(R) \in \mathbb{R}^{m \times n}$?

- Let $C = \{x \in \mathbb{R}^n \mid x_i > 0 \forall i\}$ and define $d : C \times C \rightarrow [0, \infty[$ by

$$d(x, y) := \sum_{i=1}^n \frac{(x_i - y_i)^2}{x_i y_i}.$$

Which of the axioms of a metric are fulfilled and which are not?

- Let

$$A = \begin{pmatrix} 1 & 0 & \cdots & 0 \\ \vdots & \ddots & \ddots & \vdots \\ \vdots & & \ddots & \vdots \\ 1 & \cdots & \cdots & 1 \end{pmatrix} \in \mathbb{R}^{n \times n}.$$

Calculate $\|A\|_{1 \rightarrow 1}$ (i.e. the operator norm of A when \mathbb{R}^n is equipped with the 1-norm).

- Let $A \in \mathbb{R}^{n \times n}$ and define $F : \mathbb{R}^{m \times n} \rightarrow \mathbb{R}^{m \times m}$ by $F(R) = RAR^T$. Calculate the derivative $DF(R)[H]$!
- Give a definition of a norm $\|\cdot\|_{\text{mynorm}}$ on \mathbb{R}^2 which fulfills $\left\| \begin{pmatrix} 1 \\ 0 \end{pmatrix} \right\|_{\text{mynorm}} = 10$ and $\left\| \begin{pmatrix} 0 \\ 1 \end{pmatrix} \right\|_{\text{mynorm}} = 1$.
- Let $F : \mathbb{R}^n \rightarrow \mathbb{R}$ be defined by $F(x) = \sqrt{\langle a, x \rangle}$ for $a \in \mathbb{R}^n$. Calculate $\nabla F(x)$ at some x with $\langle a, x \rangle > 0$.
- We define a map from \mathbb{R}^2 to \mathbb{R} by $\|(x, y)\|_* := |x - y|$. Argue why this is *not* a norm on \mathbb{R}^2 .
- Let $a_i \in \mathbb{R}^n$, $i = 1, \dots, m$ and $F : \mathbb{R}^n \rightarrow \mathbb{R}$ be defined by $F(x) = \sum_{i=1}^m (\langle a_i, x \rangle)^3$. Calculate $\nabla F(x)$.

10. Let $n \in \mathbb{N}$ and consider the map

$$\begin{aligned}\mathbb{R}^{n \times n} &\rightarrow [0, \infty) \\ A &\mapsto F(A) := (\operatorname{Tr}(A^T A))^{1/2}.\end{aligned}$$

(a) Show that $F(A)$ is positive definite.

Hint: You may freely use that there are an invertible matrix $P \in \mathbb{R}^{n \times n}$ and $\lambda_1, \lambda_2, \dots, \lambda_n \in [0, \infty)$ such that $A^T A = P^{-1} D P$ with the diagonal matrix

$$D = \operatorname{diag}(\lambda_1, \dots, \lambda_n) = \begin{pmatrix} \lambda_1 & 0 & \cdots & 0 \\ 0 & \lambda_2 & \cdots & 0 \\ \vdots & \ddots & \ddots & \vdots \\ 0 & \cdots & \cdots & \lambda_n \end{pmatrix} \in \mathbb{R}^{n \times n}.$$

(b) Show that $F(A)$ is homogeneous.

(c) Show the triangle inequality $F(A + B) \leq F(A) + F(B)$.

Recall also the Cauchy–Schwarz inequality

$$\left| \sum_{j=1}^n a_j b_j \right| \leq \left(\sum_{j=1}^n a_j^2 \right)^{1/2} \left(\sum_{j=1}^n b_j^2 \right)^{1/2}$$

for all $a_1, \dots, a_n, b_1, \dots, b_n \in \mathbb{R}$.

(d) Let $x, y \in \mathbb{R}^n$ and recall the notation $\|x\|_2 := (\sum_{j=1}^n |x_j|^2)^{1/2}$. Show that $F(x y^T) = \|x\|_2 \|y\|_2$ of the matrix $x y^T \in \mathbb{R}^{n \times n}$.

11. Let $n = 2$ and consider the map

$$\begin{aligned}\mathbb{R}^{2 \times 2} &\rightarrow \mathbb{R} \\ A = \begin{pmatrix} a_{11} & a_{12} \\ a_{21} & a_{22} \end{pmatrix} &\mapsto G(A) := a_{11}a_{22} - a_{21}a_{12}.\end{aligned}$$

Note that $G(A)$ is just the determinant of A .

(a) Show that for $h \in \mathbb{R}$ the derivative $DG(A)[h\mathbf{1}_2]$ along $h\mathbf{1}_2 = \begin{pmatrix} h & 0 \\ 0 & h \end{pmatrix}$ is

$$DG(A)[h\mathbf{1}_2] = h \operatorname{Tr}(A) = h(a_{11} + a_{22}).$$

(b) Let $A = \begin{pmatrix} 1 & 2 \\ 3 & 4 \end{pmatrix}$. Compute $DG(A)[h\mathbf{1}_2]$.

Possible ways so solve the problems:

1. The claim is true: We could (for example) use that the trace is invariant under cyclic permutations and get

$$\langle A^T, B^T \rangle = \text{Tr}(A^T B) = \text{Tr}(B A^T) = \langle B, A \rangle = \langle A, B \rangle.$$

One could also use the sum formula:

$$\langle A^T, B^T \rangle = \sum_{k=1}^m \sum_{j=1}^n (A^T)_{jk} (B^T)_{jk} = \sum_{k=1}^m \sum_{j=1}^n A_{kj} B_{kj} = \langle A, B \rangle.$$

2. (a) We calculate

$$\begin{aligned} F(R+H) &= \text{Tr}((R+H)(R+H)^T) \\ &= \text{Tr}(RR^T) + \text{Tr}(RH^T) + \text{Tr}(HR^T) + \text{Tr}(HH^T) \end{aligned}$$

and thus

$$F(R+H) - F(R) = \text{Tr}(RH^T) + \text{Tr}(HR^T) + \text{Tr}(HH^T)$$

Since $\text{Tr}(HH^T)/\|H\| \rightarrow 0$ for $H \rightarrow 0$ we get

$$DF(R)[H] = \text{Tr}(RH^T) + \text{Tr}(HR^T).$$

(Could further be simplified to $DF(R)[H] = 2\text{Tr}(RH^T)$ or $= 2\text{Tr}(HR^T)$ or $= 2\text{Tr}(H^T R)$ or $= 2\text{Tr}(R^T H)$)

- (b) By 1. and $\text{Tr}(A) = \text{Tr}(A^T)$ we have $DF(R)[H] = \text{Tr}(RH^T) + \text{Tr}(HR^T) = 2\text{Tr}(R^T H)$. By the definition of the inner product for matrices we get $DF(R)[H] = 2\langle H, R \rangle$ and thus $\nabla F(R) = 2R$.

3. Symmetry is fulfilled:

$$d(x, y) = \sum_{i=1}^n \frac{(x_i - y_i)^2}{x_i y_i} = \sum_{i=1}^n \frac{(y_i - x_i)^2}{y_i x_i} = d(y, x).$$

Positivity and definiteness is fulfilled as well:

$$\begin{aligned} d(x, y) &\geq 0 \text{ since } x_i \geq 0, & d(x, y) = 0 &\iff \text{for all } i: \frac{(x_i - y_i)^2}{x_i y_i} = 0 \\ & & &\iff \text{for all } i: (x_i - y_i)^2 = 0 \\ & & &\iff \text{for all } i: x_i = y_i. \end{aligned}$$

The triangle inequality is not fulfilled: We consider $n = 1$

$$\begin{aligned} d(1, 2) &= (1 - 2)^2/2 = \frac{1}{2}, \\ d(2, 3) &= (2 - 3)^2/3 = \frac{1}{3} \end{aligned}$$

but

$$d(1, 3) = (1 - 3)^2/3 = \frac{4}{3} > \frac{1}{2} + \frac{1}{3} = d(1, 2) + d(2, 3).$$

4. The norm $\|A\|_{1 \rightarrow 1}$ is the column sum norm, more precisely, the maximal 1-norm of the columns. The k -th column has 1-norm k , and hence the maximum is achieved at $k = n$ and we have $\|A\|_{1 \rightarrow 1} = n$.

5. We calculate

$$\begin{aligned} F(R+H) &= (R+H)^T A (R+H) = R^T A (R+H) + H^T A (R+H) \\ &= R^T A R + R^T A H + H^T A R + H^T A H \\ &= F(R) + R^T A H + H^T A R + H^T A H. \end{aligned}$$

Since $\|H^T A H\|/\|H\| \leq \|H^T\| \|A\| \|H\|/\|H\| = \|H^T\| \|A\| \rightarrow 0$ for $H \rightarrow 0$ and $H \mapsto R^T A H + H^T A R$ is linear in H we get

$$DF(R)[H] = R^T A H + H^T A R.$$

6. We could, for example, define

$$\left\| \begin{pmatrix} x \\ y \end{pmatrix} \right\|_{\text{mynorm}} := 10|x| + |y|.$$

(Another possibility would be $\left\| \begin{pmatrix} x \\ y \end{pmatrix} \right\|_{\text{mynorm}} := \sqrt{100|x|^2 + |y|^2}$, and there infinitely many more...)

7. We calculate

$$F(x+h) = \sqrt{\langle a, x \rangle + \langle a, h \rangle}.$$

Now we use differentiability of the function $g(t) = \sqrt{t}$: it holds that

$$\sqrt{t+\varepsilon} = g(t+\varepsilon) = g(t) + g'(t)\varepsilon + \varphi(\varepsilon) = \sqrt{t} + \frac{1}{2\sqrt{t}}\varepsilon + \varphi(\varepsilon)$$

with $\varphi(\varepsilon)/\varepsilon \rightarrow 0$ for $\varepsilon \rightarrow 0$ (this is exactly the same as doing a Taylor expansion up to first order). Using this we get

$$F(x+h) = \sqrt{\langle a, x \rangle + \langle a, h \rangle} = \sqrt{\langle a, x \rangle} + \frac{1}{2\sqrt{\langle a, x \rangle}}\langle a, h \rangle + \varphi(\langle a, h \rangle)$$

with $\varphi(\langle a, h \rangle)/\langle a, h \rangle \rightarrow 0$ for $h \rightarrow 0$. We set $\Phi(h) = \varphi(\langle a, h \rangle)$ and get from $\langle a, h \rangle \leq \|a\| \|h\|$ that

$$\frac{\Phi(h)}{\|h\|} \leq \frac{\varphi(\langle a, h \rangle)\|a\|}{\langle a, h \rangle} \rightarrow 0$$

for $h \rightarrow 0$.

Thus, we have

$$DF(x)[h] = \frac{1}{2\sqrt{\langle a, x \rangle}}\langle a, h \rangle = \left\langle \frac{1}{2\sqrt{\langle a, x \rangle}}a, h \right\rangle$$

and hence

$$\nabla F(x) = \frac{1}{2\sqrt{\langle a, x \rangle}}a.$$

8. This map is not positive definite since $\|(1, 1)\|_* = |1 - 1| = 0$.

9. One calculates

$$\begin{aligned} F(x+h) &= \sum_{i=1}^m (\langle a_i, x \rangle + \langle a_i, h \rangle)^3 \\ &= \sum_{i=1}^m \langle a_i, x \rangle^3 + 3\langle a_i, x \rangle^2 \langle a_i, h \rangle + 3\langle a_i, x \rangle \langle a_i, h \rangle^2 + \langle a_i, h \rangle^3 \\ &= F(x) + \sum_{i=1}^m 3\langle a_i, x \rangle^2 \langle a_i, h \rangle + \Phi(h). \end{aligned}$$

By Cauchy–Schwarz,

$$\begin{aligned} \frac{|\Phi(h)|}{\|h\|} &= \frac{\sum_{i=1}^m 3\langle a_i, x \rangle \langle a_i, h \rangle^2 + \langle a_i, h \rangle^3}{\|h\|} \\ &\leq \frac{\sum_{i=1}^m 3\langle a_i, x \rangle \|a_i\|^2 \|h\|^2 + \|a_i\|^3 \|h\|^3}{\|h\|} \rightarrow 0 \end{aligned}$$

for $h \rightarrow 0$. Hence,

$$DF(x)[h] = \sum_{i=1}^m 3\langle a_i, x \rangle^2 \langle a_i, h \rangle = \left\langle \sum_{i=1}^m 3\langle a_i, x \rangle^2 a_i, h \right\rangle$$

and therefore

$$\nabla F(x) = \sum_{i=1}^m 3\langle a_i, x \rangle^2 a_i.$$

10. This exercise is a little longer.

- (a) Positive definiteness: If $A = 0$, then $F(A) = 0$. If $F(A) = 0$, then $0 = \text{Tr}(A^T A) = \text{Tr}(D) = \sum_j \lambda_j$ by cyclicity of the trace. Since $\lambda_j \geq 0$ for all $j \in \{1, 2, \dots, n\}$, $\lambda_1 = \lambda_2 = \dots = \lambda_n = 0$, i.e., $A = 0$.
- (b) Homogeneity: For $\lambda \in \mathbb{R}$, we have $\|\lambda A\|_F = \sqrt{\text{Tr}((\lambda A)^T \lambda A)} = \sqrt{\lambda^2 \text{Tr}(A^T A)} = |\lambda| \|A\|_F$.
- (c) Triangle inequality: Since $\text{Tr}(A^T B) = \text{Tr}(B^T A)$ by cyclicity and $\text{Tr}(C) = \text{Tr}(C^T)$,

$$\text{Tr}(A + B)^T (A + B) = \text{Tr}(A^T A) + \text{Tr}(B^T B) + 2 \text{Tr}(A^T B).$$

Let $A = (a_{j,\ell})_{j,\ell=1}^n$, $B = (b_{j,\ell})_{j,\ell=1}^n$, $\tilde{a}_{j,\ell} = a_{\ell,j}$, and $\tilde{b}_{j,\ell} = b_{\ell,j}$. By Cauchy–Schwarz,

$$\begin{aligned} \text{Tr}(A^T B) &= \sum_{j,\ell} \tilde{a}_{j,\ell} b_{\ell,j} \leq \left(\sum_{j,\ell} (\tilde{a}_{j,\ell})^2 \right)^{1/2} \left(\sum_{j,\ell} b_{\ell,j}^2 \right)^{1/2} \\ &= \left(\sum_{j,\ell} \tilde{a}_{j,\ell} a_{\ell,j} \right)^{1/2} \left(\sum_{j,\ell} \tilde{b}_{\ell,j} b_{j,\ell} \right)^{1/2} = F(A) F(B). \end{aligned}$$

Thus,

$$F(A + B)^2 \leq F(A)^2 + F(B)^2 + 2F(A)F(B) = (F(A) + F(B))^2,$$

as desired.

- (d) Let $A = x y^T$. Then, by associativity of matrix multiplication and cyclicity of the trace,

$$\text{Tr} A^T A = \text{Tr}(y x^T x y^T) = \|x\|_2^2 \cdot \text{Tr}(y y^T) = \|x\|_2^2 \|y\|_2^2.$$

Thus, $F(x y^T) = \|x\|_2 \|y\|_2$.

11. This exercise is a little longer.

(a) We compute

$$G(A + h\mathbf{1}_2) - G(A) = h(a_{11} + a_{22}) + h^2.$$

Since

$$\lim_{h \rightarrow 0} \frac{h^2}{\|h\mathbf{1}_2\|} = 0$$

for any matrix norm (as all norms on finite dimensional vector spaces are equivalent), we obtain $DG(A)[h\mathbf{1}_2] = h \operatorname{Tr}(A) = h(a_{11} + a_{22})$.

(b) We have $DG(A)[h\mathbf{1}_2] = h \operatorname{Tr}(A) = 5h$.